James C - further work on conversion

AssemblyLanguage.thy
@@ -30,71 +30,105 @@ fun eval_assembly :: "program \<Rightarrow> assembly_state \<Rightarrow> assembl
 
 (* conversion *)
 
-fun block_size :: "assembly list \<Rightarrow> nat" where
-  "block_size [] = 0"
-| "block_size (AAssm x # as) = Suc (block_size as)"
-| "block_size (SAssm x # as) = block_size as"
-| "block_size (CAssm dst cmp jmp # as) = Suc (block_size as)"
-
 fun build_symbol_table :: "program \<Rightarrow> symbol \<rightharpoonup> nat" where
   "build_symbol_table [] s = None"
 | "build_symbol_table ((s', \<pi>) # \<Pi>) s = (
-    if s' = s 
-    then Some 0 
-    else map_option (op + (block_size \<pi>)) (build_symbol_table \<Pi> s))"
+    if s' = s then Some 0 
+    else map_option (op + (length \<pi>)) (build_symbol_table \<Pi> s))"
 
 primrec instruction_conv :: "(symbol \<rightharpoonup> nat) \<Rightarrow> assembly \<Rightarrow> instruction" where
   "instruction_conv \<rho> (AAssm x) = AInstr x"
 | "instruction_conv \<rho> (SAssm x) = AInstr (int (the (\<rho> x)))"
 | "instruction_conv \<rho> (CAssm dst cmp jmp) = CInstr dst cmp jmp"
 
-fun program_convert' :: "(symbol \<rightharpoonup> nat) \<Rightarrow> program \<Rightarrow> instruction list" where
-  "program_convert' \<rho> [] = []"
-| "program_convert' \<rho> ((s, \<pi>) # \<Pi>) = map (instruction_conv \<rho>) \<pi> @ program_convert' \<rho> \<Pi>"
+definition get_assembly :: "program \<Rightarrow> assembly list" where
+  "get_assembly \<Pi> = concat (map snd \<Pi>)"
 
 definition program_convert :: "program \<Rightarrow> instruction list" where
-  "program_convert \<Pi> = program_convert' (build_symbol_table \<Pi>) \<Pi>"
+  "program_convert \<Pi> = map (instruction_conv (build_symbol_table \<Pi>)) (get_assembly \<Pi>)"
 
-fun state_convert :: "program \<Rightarrow> assembly_state \<Rightarrow> machine_state" where
-  "state_convert \<Pi> (\<sigma>, a, d, s, \<pi>) = (\<sigma>, a, d, undefined)"
+definition get_pc :: "program \<Rightarrow> assembly list \<Rightarrow> nat set" where
+  "get_pc \<Pi> \<pi> = { the (build_symbol_table \<Pi> s) + length \<pi>'' | s \<pi>' \<pi>''. 
+    s \<in> dom (lookup \<Pi>) \<and> lookup \<Pi> s = Some \<pi>' \<and> \<pi>' = \<pi>'' @ \<pi> }"
+
+definition get_block_addr :: "program \<Rightarrow> symbol \<Rightarrow> int" where
+  "get_block_addr \<Pi> s = int (the (build_symbol_table \<Pi> s))"
+
+fun state_convert :: "program \<Rightarrow> assembly_state \<Rightarrow> machine_state set" where
+  "state_convert \<Pi> (\<sigma>, a, d, s, \<pi>) = 
+    (\<lambda>pc. (\<sigma>, a, d, pc)) ` get_pc \<Pi> \<pi> \<union> (\<lambda>pc. (\<sigma>, get_block_addr \<Pi> s, d, pc)) ` get_pc \<Pi> \<pi>"
 
 (* conversion correctness *)
 
-lemma [simp]: "eval_assembly \<Pi> \<sigma> = Some \<sigma>\<^sub>1 \<Longrightarrow> 
-    iterate (eval (program_convert \<Pi>)) (state_convert \<Pi> \<sigma>) (state_convert \<Pi> \<sigma>\<^sub>1)"
+lemma [simp]: "lookup \<Pi> s = Some \<pi> \<Longrightarrow> \<exists>n. build_symbol_table \<Pi> s = Some n"
+  by (induction \<Pi> s rule: lookup.induct) auto
+
+lemma [simp]: "lookup \<Pi> s = Some \<pi> \<Longrightarrow> n < length \<pi> \<Longrightarrow> 
+    the (build_symbol_table \<Pi> s) + n < length (get_assembly \<Pi>)"
+  proof (induction \<Pi> s rule: build_symbol_table.induct)
+  case 1
+    thus ?case by simp
+  next case (2 s' \<pi>' \<Pi> s)
+    thus ?case
+      proof (cases "s' = s")
+      case True
+        with 2 show ?thesis by (simp add: get_assembly_def)
+      next case False
+        with 2 obtain m where "build_symbol_table \<Pi> s = Some m" by fastforce
+        with 2 False show ?thesis by (simp add: get_assembly_def)
+      qed
+  qed
+
+lemma [simp]: "lookup \<Pi> s = Some \<pi> \<Longrightarrow> n < length \<pi> \<Longrightarrow>  
+    get_assembly \<Pi> ! (the (build_symbol_table \<Pi> s) + n) = \<pi> ! n"
+  proof (induction \<Pi> s rule: build_symbol_table.induct)
+  case 1
+    thus ?case by simp
+  next case (2 s' \<pi>' \<Pi> s)
+    thus ?case
+      proof (cases "s' = s")
+      case True
+        with 2 show ?thesis by (simp add: get_assembly_def nth_append)
+      next case False
+        with 2 obtain m where "build_symbol_table \<Pi> s = Some m" by fastforce
+        with 2 False show ?thesis by (simp add: get_assembly_def add.assoc)      
+      qed
+  qed
+
+lemma [simp]: "pc \<in> get_pc \<Pi> (a # \<pi>) \<Longrightarrow> 
+    program_convert \<Pi> ! pc = instruction_conv (build_symbol_table \<Pi>) a"
+  by (auto simp add: get_pc_def program_convert_def)
+
+lemma eval_assembly_conv [simp]: "eval_assembly \<Pi> \<sigma> = Some \<sigma>\<^sub>1 \<Longrightarrow> \<sigma>' \<in> state_convert \<Pi> \<sigma> \<Longrightarrow>
+    \<exists>\<sigma>\<^sub>1'. \<sigma>\<^sub>1' \<in> state_convert \<Pi> \<sigma>\<^sub>1 \<and> eval (program_convert \<Pi>) \<sigma>' = Some \<sigma>\<^sub>1'"
   proof (induction \<Pi> \<sigma> rule: eval_assembly.induct)
   case (1 \<Pi> \<sigma> a d s)
     thus ?case by simp
   next case (2 \<Pi> \<sigma> a d s x \<pi>)
-    hence "eval_assembly \<Pi> (\<sigma>, a, d, s, AAssm x # \<pi>) = Some \<sigma>\<^sub>1" by simp
+    from 2 have "\<sigma>' \<in> (\<lambda>pc. (\<sigma>, a, d, pc)) ` get_pc \<Pi> (AAssm x # \<pi>) \<union> (\<lambda>pc. (\<sigma>, get_block_addr \<Pi> s, d, pc)) ` get_pc \<Pi> (AAssm x # \<pi>)" by simp
 
 
 
-    have "iterate (eval (program_convert \<Pi>)) (state_convert \<Pi> (\<sigma>, a, d, s, AAssm x # \<pi>)) (state_convert \<Pi> \<sigma>\<^sub>1)" by simp
-    thus ?case by simp
+    have "\<sigma>\<^sub>1' \<in> (\<lambda>pc. (\<sigma>, x, d, pc)) ` get_pc \<Pi> \<pi> \<and> eval (program_convert \<Pi>) \<sigma>' = Some \<sigma>\<^sub>1'" by simp
+    with 2 show ?case by fastforce
   next case (3 \<Pi> \<sigma> a d s x \<pi>)
-    hence "eval_assembly \<Pi> (\<sigma>, a, d, s, SAssm x # \<pi>) = Some \<sigma>\<^sub>1" by simp
-
-
-
-    have "iterate (eval (program_convert \<Pi>)) (state_convert \<Pi> (\<sigma>, a, d, s, SAssm x # \<pi>)) (state_convert \<Pi> \<sigma>\<^sub>1)" by simp
     thus ?case by simp
   next case (4 \<Pi> \<sigma> a d s dst cmp jmp \<pi>)
-    hence "eval_assembly \<Pi> (\<sigma>, a, d, s, CAssm dst cmp jmp # \<pi>) = Some \<sigma>\<^sub>1" by simp
-
-
-
-    have "iterate (eval (program_convert \<Pi>)) (state_convert \<Pi> (\<sigma>, a, d, s, CAssm dst cmp jmp # \<pi>)) (state_convert \<Pi> \<sigma>\<^sub>1)" by simp
     thus ?case by simp
   qed
 
-theorem [simp]: "iterate (eval_assembly \<Pi>) \<sigma> \<sigma>\<^sub>1 \<Longrightarrow> 
-    iterate (eval (program_convert \<Pi>)) (state_convert \<Pi> \<sigma>) (state_convert \<Pi> \<sigma>\<^sub>1)"
-  proof (induction "eval_assembly \<Pi>" \<sigma> \<sigma>\<^sub>1 rule: iterate.induct) 
+theorem [simp]: "iterate (eval_assembly \<Pi>) \<sigma> \<sigma>\<^sub>1 \<Longrightarrow> \<sigma>' \<in> state_convert \<Pi> \<sigma> \<Longrightarrow>
+    \<exists>\<sigma>\<^sub>1'. \<sigma>\<^sub>1' \<in> state_convert \<Pi> \<sigma>\<^sub>1 \<and> iterate (eval (program_convert \<Pi>)) \<sigma>' \<sigma>\<^sub>1'"
+  proof (induction "eval_assembly \<Pi>" \<sigma> \<sigma>\<^sub>1 arbitrary: \<sigma>' rule: iterate.induct)
   case iter_refl
-    thus ?case by simp
-  next case iter_step
     thus ?case by fastforce
+  next case (iter_step \<sigma> \<sigma>\<^sub>1 \<sigma>\<^sub>2)
+    then obtain \<sigma>\<^sub>1' where S: "\<sigma>\<^sub>1' \<in> state_convert \<Pi> \<sigma>\<^sub>1 \<and> iterate (eval (program_convert \<Pi>)) \<sigma>' \<sigma>\<^sub>1'" 
+      by blast
+    with iter_step eval_assembly_conv obtain \<sigma>\<^sub>2' where
+      "\<sigma>\<^sub>2' \<in> state_convert \<Pi> \<sigma>\<^sub>2 \<and> eval (program_convert \<Pi>) \<sigma>\<^sub>1' = Some \<sigma>\<^sub>2'" by blast
+    with S have "\<sigma>\<^sub>2' \<in> state_convert \<Pi> \<sigma>\<^sub>2 \<and> iterate (eval (program_convert \<Pi>)) \<sigma>' \<sigma>\<^sub>2'" by fastforce
+    thus ?case by blast
   qed
 
 end
